src/vminus/Classes.v
@@ -1,0 +1,11 @@
+Require Import String.
+
+Definition err (A : Type) : Type := (string + A)%type.
+Definition err_bind {A B : Type}
+           (MA : err A) (f: A -> B) (MB : err B) :=
+  match MA with
+  | inl err => inl err
+  | inr x => inr (f x)
+  end.
+Definition err_ret {A : Type} (a : A) : err A :=
+  inr a.
