src/vminus/ListCFG.v
@@ -1,0 +1,267 @@
+Require Import Arith.
+Require Import List.
+Import ListNotations.
+
+Require Import Vminus.Util.
+Require Import Vminus.Vminus.
+
+Require Import Vminus.CFG.
+
+(** *** List-based CFG Implementation *)
+
+(**  One possible implementation of cfgs *)
+
+Module ListCFG <: CFG.
+  Definition block := (lbl * list insn)%type.
+  Definition t := (lbl * list block)%type.
+  Local Notation cfg := t.
+
+  Definition entry_block : cfg -> lbl := @fst _ _.
+
+  Inductive wf_cfg' : cfg -> Prop :=
+    wf_cfg_intro : forall l bs,
+    NoDup (map (@fst _ _) bs) ->
+    NoDup (flat_map (fun b => map (@fst _ _) (snd b)) bs) ->
+    In l (map (@fst _ _) bs) ->
+    ~ In [] (map (@snd _ _) bs) ->
+    wf_cfg' (l, bs).
+
+  (* hack around some limitation re inductive types & parameters *)
+  Definition wf_cfg := wf_cfg'.
+
+  Lemma wf_cfg_block_len : forall g, wf_cfg g ->
+    forall l is, In (l, is) (snd g) -> length is <> 0.
+  Proof.
+    inversion 1. intros. destruct is; simpl; auto. 
+    contradict H2. 
+    eapply in_map with (f:=@snd _ _) in H5. auto.
+  Qed.
+
+  Definition wf_pc (g:cfg) (p:pc) : Prop :=
+    let (l, n) := p in
+    exists is i, In (l, is) (snd g) /\ Nth i is n.
+
+  Definition tmn_pc (g:cfg) (p:pc) : Prop :=
+    let (l, n) := p in
+    exists is, In (l, is) (snd g) /\ n = pred (length is).
+
+  Definition insn_at_pc (g:cfg) (p:pc) (i:insn) : Prop :=
+    let (l, n) := p in
+    exists is, In (l, is) (snd g) /\ Nth i is n.
+    
+  Definition uid_at_pc (g:cfg) (p:pc) (uid:uid) : Prop :=
+    exists c, insn_at_pc g p (uid, c).
+
+  Lemma wf_pc_insn : forall g, wf_cfg g ->
+    forall p, wf_pc g p -> exists i, insn_at_pc g p i.
+  Proof.
+    unfold wf_pc, insn_at_pc. destruct p; intros. 
+    decompose [ex and] H0. eauto.
+  Qed.
+
+  Lemma wf_pc_tmn : forall g, wf_cfg g ->
+    forall p, wf_pc g p -> exists p', tmn_pc g p' /\ le_pc p p'.
+  Proof.
+    unfold wf_pc, tmn_pc. destruct p. intros.
+    decompose [ex and] H0. 
+    exists (t0, pred (length x)). split. eauto.
+    constructor. 
+    apply PeanoNat.Nat.lt_le_pred.
+    eapply Nth_length; eauto.
+  Qed.
+
+  Lemma wf_pc_le_tmn : forall g, wf_cfg g ->
+    forall p', tmn_pc g p' -> forall p, le_pc p p' -> wf_pc g p.
+  Proof.
+    unfold wf_pc, tmn_pc. intros. destruct p, p'.
+    decompose [ex and] H0. exists x.
+
+    destruct x. apply wf_cfg_block_len in H3; auto. contradict H3; auto.
+    inversion H1; subst. apply le_lt_n_Sm in H5. 
+    erewrite <- S_pred in H5. 
+    apply length_Nth in H5 as [? ?]. 
+    eexists. split; eauto. eauto.
+  Qed.
+
+  Lemma wf_entry : forall g, wf_cfg g ->
+    wf_pc g (block_entry (entry_block g)).
+  Proof.
+    unfold wf_pc. inversion 1. simpl.
+    apply in_map_iff in H2 as [[? ?] [? ?]].
+    destruct l0.
+    exfalso. pose proof (wf_cfg_block_len g H t0 []) as contra. 
+    subst g; simpl in *. apply contra; auto.
+    eexists. eexists. 
+    simpl in *. subst l. split; eauto.
+    simpl; eauto.
+  Qed.
+
+  Lemma insn_at_pc_func : forall g, wf_cfg g ->
+    functional (insn_at_pc g).
+  Proof. 
+    unfold functional, insn_at_pc. inversion 1. destruct a.
+    intros b1 b2 [is1 [Hin1 Hnth1]] [is2 [Hin2 Hnth2]].
+    cut (is1 = is2). intro; subst is2. eapply Nth_eq; eauto.
+    eapply NoDup_assoc_func; eauto.
+  Qed.
+
+  Lemma uid_at_pc_inj : forall g, wf_cfg g ->
+    injective (uid_at_pc g).
+  Proof.
+    unfold injective, uid_at_pc, insn_at_pc. inversion 1.
+    intros [l1 n1] [l2 n2] uid [c1 [is1 [Hin1 Hnth1]]] [c2 [is2 [Hin2 Hnth2]]].
+    cut ((l1, is1) = (l2, is2)).
+    intro Heq. inversion Heq; clear Heq. f_equal.
+    eapply NoDup_flat_map__NoDup in H1; eauto.
+    change is1 with (snd (l1, is1)) in Hnth1.
+    change is2 with (snd (l2, is2)) in Hnth2.
+    subst; eapply NoDup_nth_inj; eauto. 
+
+    set (f1 b := map (@fst _ _) (snd b)) in *.
+    apply (NoDup_flat_map (l1, is1) (l2, is2) uid f1 bs); auto.
+    unfold f1; simpl. 
+    apply in_map_iff. exists (uid, c1); eauto using Nth_In.
+    apply in_map_iff. exists (uid, c2); eauto using Nth_In.
+  Qed.
+
+  (** ** Working with ListCFG. *)
+
+  (** Adds the given instruction list as a block labeled [l]. *)
+
+  Definition update (bs:list block) (l:lbl) (is:list insn) : list block :=
+    (l, is)::bs.
+
+  (** Lookup the block in the list. *)
+
+  Definition lookup (bs:list block) (l:lbl) : option (list insn) :=
+    assoc Lbl.eq_dec l bs.
+
+  (** ** Simple lemmas about CFG modifications. *)
+
+  Lemma update_eq :
+    forall (is : list insn) (l1 l2 : lbl) (bs : list block),
+      l1 = l2 -> lookup (update bs l1 is) l2 = Some is.
+  (* FOLD *)
+  Proof.
+    intros; unfold update, lookup.
+    subst. simpl. destruct (Lbl.eq_dec l2 l2); tauto.
+  Qed.
+  (* /FOLD *)
+
+  Lemma update_neq :
+    forall (l1 l2 : lbl) (is : list insn) (bs: list block),
+      l1 <> l2 -> lookup (update bs l1 is) l2 = lookup bs l2.
+  (* FOLD *)
+  Proof.
+    intros; subst; simpl.
+    destruct (Lbl.eq_dec l2 l1); subst; tauto.
+  Qed.
+  (* /FOLD *)
+
+  (* Added *)
+  Fixpoint find_block {A : Type} (lst : list (lbl * A)) (trgt_label : lbl) :=
+    match lst with
+    | [] => None
+    | (label, data) :: other_blks =>
+      if Lbl.eq_dec label trgt_label then
+        Some data 
+      else find_block other_blks trgt_label
+    end.
+      
+  Definition fetch (g : cfg) (p: pc): option insn :=
+    let '(entry_label, blocks) := g in
+    let '(trgt_block, offset) := p in
+    match (find_block blocks trgt_block) with
+    | Some found_block => nth_error found_block offset
+    | None => None
+    end.
+  
+  Lemma find_block_ok: forall (blks: list (lbl * list insn)) found_instrs (label: lbl),
+      NoDup (List.map fst blks) -> 
+      find_block blks label = Some found_instrs <->
+      In (label, found_instrs) blks.
+  Proof.
+    intros blks found_instrs label nodups.
+    induction blks as [| blk other_blks].
+    { simpl; split; intros H; inversion H. }
+    { simpl; destruct blk as [this_label this_insns].
+      destruct (Lbl.eq_dec this_label label) as [label_eq | label_neq].
+      { split; intros H;
+          [inversion H as [found_this] | idtac].
+        - subst; left; auto.
+        - destruct H as [found_here | found_in_others].
+          + inversion found_here; subst; trivial.
+          + simpl in nodups.
+            (* Want the following as lemma *)
+            replace (this_label :: map fst other_blks) with
+                ([] ++ (this_label :: map fst other_blks)) in nodups
+              by auto.
+            apply NoDup_remove in nodups.
+            inversion nodups as [? not_found_in_others].
+            apply in_map with (f := fst) in found_in_others.
+            simpl in found_in_others.
+            contradiction not_found_in_others.
+            simpl; subst; apply found_in_others.
+      } 
+      { simpl in nodups.
+        replace (this_label :: map fst other_blks) with
+            ([] ++ (this_label :: map fst other_blks)) in nodups
+          by auto.
+        apply NoDup_remove in nodups.
+        inversion nodups as [nodups_in_others this_label_in_others].
+        generalize (IHother_blks nodups_in_others) as IH; intros IH.
+        rewrite IH.
+        split; auto.
+        intros [Hcontra | ?]; auto.
+        contradiction label_neq.
+        inversion Hcontra; auto.
+      }
+    } 
+  Qed.
+      
+  Lemma find_block_iff_in_cfg: forall entry_label blks trgt_label trgt_offset i,
+      NoDup (map fst blks) -> 
+      fetch (entry_label, blks) (trgt_label, trgt_offset) = Some i <->
+      exists instrs, In (trgt_label, instrs) blks /\ Nth i instrs trgt_offset.
+  Proof.
+    intros entry_label blks trgt_label trgt_offset i nodup.
+    unfold fetch.
+    destruct (find_block blks trgt_label) eqn:found.
+    { apply find_block_ok in found; auto.
+      split.
+      { intros H; exists l; split; trivial.
+        rewrite nth_error_iff_Nth in H.
+        trivial.
+      }
+      { intros [instrs [trgt_blk_found trgt_instr_found]].
+        rewrite <- nth_error_iff_Nth in trgt_instr_found.
+        replace l with instrs; auto.
+        eapply NoDup_assoc_func.
+        apply nodup.
+        apply trgt_blk_found.
+        trivial.
+      }         
+    } 
+    { split; intros H; [inversion H | idtac].
+      destruct H as [instrs [trgt_label_found trgt_instr_found]].
+      rewrite <- nth_error_iff_Nth in trgt_instr_found.
+      rewrite <- find_block_ok in trgt_label_found; auto.
+      rewrite trgt_label_found in found; inversion found.
+    }
+  Qed.
+  
+  (* Added *)
+  Lemma insn_at_pc_fetch :
+    forall g pc i, wf_cfg g ->
+              insn_at_pc g pc i <-> fetch g pc = Some i.
+  Proof.
+    intros [l blks] pc i wf_g.
+    inversion wf_g as
+        [l' blks' nodup nodup_uid l_in_blks blks_not_empty [l_l' blks_blk]].
+    destruct pc as [curr_label curr_offset].
+    rewrite find_block_iff_in_cfg; auto.
+    simpl.
+    split; auto.
+  Qed.      
+    
+End ListCFG.
